Cleanup

theories/Categories.v
@@ -10,6 +10,8 @@ Require Import Coq.Unicode.Utf8.
 Require Import Coq.Classes.SetoidClass.
 Require Import Coq.Program.Tactics.
 Require Import Coq.Lists.List.
+Require Coq.Vectors.Fin.
+Require Coq.Vectors.Vector.
 
 Import IfNotations.
 Import List.ListNotations.
@@ -26,10 +28,135 @@ Implicit Types x y: var.
 Implicit Type ρ: subst.
 
 Module Import Hor.
-  Definition Hor Γ Γ' := { ρ | Jp ρ Γ Γ' }.
+  Fixpoint zip {A B} (l: list A) (r: list B): list (A * B) :=
+    match l, r with
+    | cons a l', cons b r' => cons (a, b) (zip l' r')
+    | _, _ => nil
+    end.
+
+  Lemma zip_fst_snd {A B} (l: list (A * B)): zip (List.map fst l) (List.map snd l) = l.
+  Proof.
+    induction l.
+    1: reflexivity.
+    cbn.
+    rewrite IHl.
+    destruct a.
+    reflexivity.
+  Qed.
+
+  Definition Hor A τ := {
+      f: list intro → intro |
+      ∀ Γ vs, List.Forall2 (λ v τ, Γ ⊢ v ⇐ τ) vs A → Γ ⊢ f vs ⇐ τ
+    } .
+
+  #[refine]
+  Instance Hor_Setoid τs τ: Setoid (Hor τs τ) := {
+      equiv f g := ∀ vs, proj1_sig f vs = proj1_sig g vs
+  }.
+  Proof.
+    exists.
+    - intro.
+      reflexivity.
+    - intro.
+      symmetry.
+      eauto.
+    - intros ? ? ? p q ?.
+      rewrite p, q.
+      reflexivity.
+  Defined.
 
   #[program]
-  Definition id A: Hor A A := [].
+   Definition id τ: Hor [τ] τ := λ vs, match vs with
+                                       | [v] => v
+                                       | _ => v_tt
+                                       end.
+
+  Next Obligation.
+  Proof.
+    inversion H.
+    subst.
+    inversion H4.
+    subst.
+    auto.
+  Qed.
+
+
+  #[program]
+   Definition cut {A B C} (f: Hor (C :: A) B) (g: Hor A C): Hor A B :=
+    λ vs, proj1_sig f (proj1_sig g vs :: vs).
+
+  Next Obligation.
+  Proof.
+    destruct f as [f fp], g as [g gp].
+    cbn.
+    apply fp.
+    constructor.
+    1: apply gp.
+    all: auto.
+  Qed.
+
+  Infix "∘" := cut (at level 30).
+
+  #[program]
+  Definition pure_elim A xs V τ: zip xs A ⊢ V ⇒ τ → Hor A τ := λ _ vs, Term.eval_elim (zip xs vs) V.
+
+  Next Obligation.
+  Proof.
+    apply (Term.eval_elim_preserves j).
+    clear j V.
+    generalize dependent xs.
+    induction H.
+    1: destruct xs.
+    1,2: constructor.
+    destruct xs.
+    1: cbn; constructor.
+    cbn.
+    constructor.
+    1: auto.
+    eapply IHForall2.
+  Qed.
+
+  #[program]
+  Definition pure A xs v τ: zip xs A ⊢ v ⇐ τ → Hor A τ := λ _ vs, Term.eval (zip xs vs) v.
+
+  Next Obligation.
+  Proof.
+    apply (Term.eval_preserves j).
+    clear j v.
+    generalize dependent xs.
+    induction H.
+    1: destruct xs.
+    1,2: constructor.
+    destruct xs.
+    1: cbn; constructor.
+    cbn.
+    constructor.
+    1: auto.
+    eapply IHForall2.
+  Qed.
+
+  Fixpoint mt (n: nat): list var.
+  Proof.
+    destruct n.
+    - apply [].
+    - apply cons.
+      + apply 0.
+      + auto.
+  Defined.
+
+  #[program]
+   Definition head τ A: Hor (τ :: A) τ :=
+    let x := 0 in
+    pure_elim (τ :: A) (x :: mt (length A)) (V_var x) τ _.
+
+  Next Obligation.
+  Proof.
+    constructor.
+    constructor.
+  Qed.
+
+  #[program]
+  Definition tt A: Hor A t_unit := pure A (mt (length A)) v_tt t_unit _.
 
   Next Obligation.
   Proof.
@@ -37,52 +164,70 @@ Module Import Hor.
   Qed.
 
   #[program]
-  Definition compose {A B C} (f: Hor B C) (g: Hor A B): Hor A C := g ++ f.
-
-  Next Obligation.
-  Proof.
-    destruct g as [g gp].
-    destruct f as [f fp].
-    cbn.
-    generalize dependent C.
-    generalize dependent B.
-    generalize dependent A.
-    generalize dependent f.
-    generalize dependent g.
-    intro g.
-    induction g.
-    all: cbn.
-    all: intros.
-    - inversion gp.
-      auto.
-    - inversion gp.
-      subst.
-      econstructor.
-      1: apply H1.
-      eauto.
-  Qed.
-
-  Infix "∘" := compose (at level 30).
-
-  #[program]
-  Definition pure {x Γ t} (p: { v | Γ ⊢ v ⇐ t}): Hor Γ [(x, t)] := [(x, proj1_sig p)].
-
-  Next Obligation.
-  Proof.
-    apply (Jp_cut _ _ _ _ _ _ _ H (Jp_id [_])).
-  Qed.
-
-  #[program]
-  Definition fanout {Γ} {x y z A B}: x ≠ y → Hor ((x, A) :: (y, B) :: Γ) [(z, A * B)] := λ _,
-    pure (v_fanout (η A (V_var x)) (η B (V_var y))).
+  Definition fanout A B C: Hor (A :: B :: C) (A * B) :=
+      let x: var := 0 in
+      let y: var := 1 in
+      pure (A :: B :: C)
+           (x :: y:: mt (length C))
+           (v_fanout (η A (V_var x)) (η B (V_var y)))
+           (A * B)
+           _.
 
   Next Obligation.
   Proof.
     econstructor.
     all: apply Term.η_preserve.
-    all: constructor.
-    all: repeat constructor.
-    auto.
+    - repeat constructor.
+    - repeat constructor.
+      auto.
+  Qed.
+
+  #[program]
+   Definition fst {A B C}: Hor ((A * B) :: C) A :=
+    let x: var := 0 in
+    pure_elim (A * B :: C)
+         (x :: mt (length C))
+         (V_fst (V_var x))
+         A
+         _.
+
+  Next Obligation.
+  Proof.
+    repeat econstructor.
+  Qed.
+
+  #[program]
+   Definition snd {A B C}: Hor ((A * B) :: C) B :=
+    let x: var := 0 in
+    pure (A * B :: C)
+         (x :: mt (length C))
+         (η B (V_snd (V_var x)))
+         B
+         _.
+
+  Next Obligation.
+  Proof.
+    apply Term.η_preserve.
+    repeat econstructor.
+  Qed.
+
+  Lemma tt_f {A B} {f: Hor A B}: tt _ ∘ f == tt _.
+  Proof.
+    destruct f as [f fp].
+    cbn.
+    intro.
+    reflexivity.
+  Qed.
+
+  Lemma fst_fanout {A B C}: fst ∘ fanout A B C == head _ _.
+  Proof.
+    intro.
+    cbn.
+    destruct vs.
+    all: cbn.
+    
+    intro.
+    reflexivity.
   Qed.
 End Hor.
 
